games/Composition.v
@@ -1,0 +1,250 @@
+Require Import LogicalRelations.
+Require Import List.
+Require Import Classical.
+Require Import Events.
+Require Import Smallstep.
+Require Import Behaviors.
+Require Import LTS.
+Require Import Trees.
+Require Import GameSemantics.
+Require Import ModuleSemantics.
+Require Import Classical.
+
+
+(** * Resolution operator *)
+
+Module Res.
+
+  (** ** Core transition system *)
+
+  Section RESOLVE.
+    Context {li : language_interface}.
+    Context (dom : query li -> bool).
+    Context {A} (α : lts (option (move (li -o li))) A) (a0 : A).
+
+    Definition state : Type := list A.
+
+    Definition fcall q := Some (@qm (li -o li) (inr q)).
+    Definition fret  r := Some (@rm (li -o li) (inr r)).
+    Definition xcall q := Some (@rm (li -o li) (inl q)).
+    Definition xret  r := Some (@qm (li -o li) (inl r)).
+
+    Definition observable (at_outer_layer : Prop) (m : option (move (li -o li))) :=
+      match m with
+        | Some (rm (inr r)) => at_outer_layer
+        | Some (rm (inl q)) => dom q = false
+        | _ => True
+      end.
+
+    Inductive step : option (move (li -o li)) -> relation state :=
+      | step_observable m a a' ks:
+          observable (ks = nil) m ->
+          α m a a' ->
+          step m (a :: ks) (a' :: ks)
+      | step_push q a k aq ks :
+          dom q = true ->
+          α (xcall q) a k ->
+          α (fcall q) a0 aq ->
+          step None (a :: ks) (aq :: k :: ks)
+      | step_pop r a a' k ar ks :
+          α (fret r) a a' ->
+          α (xret r) k ar ->
+          step None (a :: k :: ks) (ar :: ks).
+
+  End RESOLVE.
+
+  (** ** Core commutation theorem *)
+
+  Definition etc {li} (m : option (move (li -o li))) : bool :=
+    match m with Some m => tc m | None => true end.
+
+  Section COMMUT.
+    Context {li} (L : semantics (li -o li)) (dom : query li -> bool).
+
+    Inductive res_commut_st ks : rel _ (option (ModuleSemantics.Res.state L)) :=
+      | res_commut_st_none:
+          res_commut_st ks None None
+      | res_commut_st_some s:
+          res_commut_st ks s (Some (s, ks)).
+
+    Hint Constructors res_commut_st.
+
+    Inductive res_commut_sim : rel _ _ :=
+      | res_commut_sim_waiting k ks :
+          res_commut_sim
+            (Behavior.waiting L k :: map (Behavior.waiting L) ks)
+            (Behavior.waiting (Res.semantics L dom) (Res.liftk L k ks))
+      | res_commut_sim_running_some t s rs ks :
+          res_commut_st ks s rs ->
+          res_commut_sim
+            (Behavior.running L t s :: map (Behavior.waiting L) ks)
+            (Behavior.running (Res.semantics L dom) t rs)
+      | res_commut_sim_wrong ks :
+          res_commut_sim
+            (Behavior.wrong L :: ks)
+            (Behavior.wrong (Res.semantics L dom)).
+
+    Lemma commut_observable r ks :
+      ModuleSemantics.Res.observable L dom r ks <->
+      Res.observable dom (map (Behavior.waiting L) ks = nil) (Some (rm r)).
+    Proof.
+      simpl. unfold ModuleSemantics.Res.observable.
+      destruct r.
+      - reflexivity.
+      - split.
+        + intro. subst. reflexivity.
+        + destruct ks; simpl; congruence.
+    Qed.
+
+    Lemma apply_cont_exists k q:
+      exists s, apply_cont L k q s.
+    Proof.
+      destruct (classic (exists s, k q s)) as [[s Hs] | Hns].
+      - exists (Some s). constructor. eauto.
+      - exists None. constructor. eauto.
+    Qed.
+
+    Lemma commut_goes_wrong s ks:
+      (Nostep L s /\ forall r k, ~ final_state L s r k) <->
+      (Nostep (Res.semantics L dom) (Some s, ks) /\
+       forall r k, ~ final_state (Res.semantics L dom) (Some s, ks) r k).
+    Proof.
+      split.
+      - intros [Hns Hnf]. split.
+        + intros t s' Hs'.
+          inversion Hs'; clear Hs'; subst.
+          * eapply Hns; eauto.
+          * eapply Hnf; eauto.
+          * eapply Hnf; eauto.
+        + intros r k Hs.
+          inversion Hs; clear Hs; subst.
+          eapply Hnf; eauto.
+      - intros [Hns Hnf]. split.
+        + intros t s' Hs'.
+          eapply Hns. constructor. eauto.
+        + intros r k Hs.
+          destruct r as [q | r].
+          * destruct (dom q) eqn:Hq.
+            -- edestruct apply_cont_exists as [s' Hs'].
+               eapply Hns. eapply Res.step_call; eauto.
+            -- eapply Hnf. constructor; eauto.
+               simpl. assumption.
+          * destruct ks.
+            -- eapply Hnf. constructor; eauto.
+               simpl. reflexivity.
+            -- edestruct apply_cont_exists as [s' Hs'].
+               eapply Hns. eapply Res.step_return; eauto.
+    Qed.
+
+    Lemma apply_cont_commut k q s ks:
+      let os := option_map (fun s => (Some s, ks)) s in
+      apply_cont L k q s ->
+      apply_cont (Res.semantics L dom) (Res.liftk L k ks) q os.
+    Proof.
+      intro; subst os.
+      destruct 1.
+      - constructor. constructor. assumption.
+      - constructor. intros s Hs. destruct Hs. eapply H; eauto.
+    Qed.
+
+    Lemma res_commut :
+      LTS.bisim res_commut_sim
+        (step dom (Behavior.step L) (Behavior.waiting L (initial_state L)))
+        (Behavior.step (Res.semantics L dom)).
+    Proof.
+      intros m s1 s2 Hs.
+      split.
+      - (* Forward *)
+        intros s1' Hs1'.
+        destruct Hs1'.
+        + (* observable step *)
+          destruct H0; inversion Hs; clear Hs; subst; simpl in H.
+          * eexists; split; constructor.
+            -- eapply apply_cont_commut; eauto.
+            -- destruct s; simpl; eauto.
+          * inversion H5; clear H5; subst.
+            eexists; split; constructor; constructor; eauto.
+          * eexists; split; constructor; eauto.
+          * inversion H5; clear H5; subst.
+            eexists; split; constructor; eauto.
+            constructor; eauto. apply commut_observable. simpl. auto.
+          * inversion H6; clear H6; subst.
+            eexists; split; constructor; eauto;
+            eapply commut_goes_wrong; eauto.
+          * inversion H4; clear H4; subst;
+            eexists; split; constructor; eauto.
+            -- intros t s' Hs'. inversion Hs'.
+            -- intros r k Hs. inversion Hs.
+        + (* push *)
+          inversion H0; clear H0; subst.
+          inversion Hs; clear Hs; subst.
+          inversion H6; clear H6; subst.
+          inversion H1; clear H1; subst.
+          change (?f ?hd :: map ?f ?tl) with (map f (hd :: tl)).
+          eexists. split.
+          * constructor. eapply Res.step_call; eauto.
+          * econstructor. destruct H4; constructor.
+        + (* pop *)
+          inversion H; clear H; subst.
+          inversion H0; clear H0; subst.
+          inversion Hs; clear Hs; subst.
+          inversion H5; clear H5; subst.
+          destruct ks0 as [ | xk xks]; try discriminate.
+          inversion H4; clear H4; subst.
+          eexists. split.
+          * constructor. eapply Res.step_return; eauto.
+          * constructor. destruct H1; constructor.
+      - (* Backward *)
+        intros s2' Hs2'.
+        destruct Hs2'; inversion Hs; clear Hs; subst.
+        + (* waiting -> running *)
+          destruct H.
+          * destruct H.
+            eexists; split; econstructor; simpl; eauto.
+            constructor. constructor; eauto.
+          * eexists; split; econstructor; simpl; eauto.
+            constructor. constructor; eauto.
+            intros s Hs. eapply H. constructor; eauto.
+        + (* running *)
+          inversion H2; clear H2; subst.
+          inversion H; clear H; subst.
+          * (* internal step *)
+            eexists; split; constructor; simpl; eauto.
+            constructor; eauto.
+          * (* call *)
+            eexists; split; [ | constructor; eauto]. simpl. econstructor.
+            -- eassumption.
+            -- constructor; eauto.
+            -- constructor; eauto.
+          * (* return *)
+            eexists. split.
+            -- eapply step_pop.
+               ++ constructor; eauto.
+               ++ constructor; eauto.
+            -- constructor; eauto.
+        + (* dequeue *)
+          eexists; split; constructor; simpl; eauto.
+          constructor.
+        + (* terminate *)
+          destruct H.
+          inversion H2; clear H2; subst.
+          apply commut_observable in H.
+          eexists; split; constructor; simpl; eauto.
+          constructor; eauto.
+        + (* go wrong *)
+          inversion H3; clear H3; subst.
+          destruct s0.
+          * edestruct (proj2 (commut_goes_wrong s ks)) as [Hns Hnf]; eauto.
+            eexists. split; constructor.
+            -- simpl. auto.
+            -- constructor; eauto.
+          * eexists. split; constructor.
+            -- simpl. auto.
+            -- constructor; eauto.
+        + inversion H1; clear H1; subst.
+          eexists; split; constructor; simpl; auto.
+          constructor.
+    Qed.
+
+  End COMMUT.
+End Res.
